concurrency/juicy/semax_safety_freelock.v
@@ -792,8 +792,9 @@ Proof.
     * repeat REWR.
       destruct (getThreadC j tp lj) eqn:Ej.
       -- destruct (cl_halted s) eqn:Halted.
-           eapply jsafeN_halted; eauto. simpl. rewrite Halted; intro Hx; inv Hx.
-           instantiate (1:=Int.zero). apply Logic.I.  
+           destruct s; inv Halted. destruct v0; inv H0. destruct c; inv H1.
+           eapply jsafeN_halted; eauto. reflexivity.
+           apply Logic.I.  
            edestruct (unique_Krun_neq(ge := ge) i j); eauto.
       -- apply jsafe_phi_age_to; auto. apply jsafe_phi_downward. assumption.
       -- intros c' Ec'; specialize (safety c' Ec'). apply jsafe_phi_bupd_age_to; auto. apply jsafe_phi_bupd_downward. assumption.
